pulse/lib/pulse/lib/Pulse.Lib.Core.fsti
@@ -58,42 +58,42 @@ val allow_ambiguous : unit
 [@@erasable]
 val slprop : Type u#4
 
-(* slprop4: slprops that can be represented in universe 4.
-Currently, just an alias to slprop, but this provides a stable universe 4 interface. *)
-[@@erasable]
-val slprop4_base : Type u#4
-val down4 (p:slprop) : slprop4_base
-val up4 (p:slprop4_base) : slprop
-let is_slprop4 (v:slprop) : prop = up4 (down4 v) == v
-val up4_is_slprop4 (p:slprop4_base) : Lemma (is_slprop4 (up4 p))
+// (* slprop4: slprops that can be represented in universe 4.
+// Currently, just an alias to slprop, but this provides a stable universe 4 interface. *)
+// [@@erasable]
+// val slprop4_base : Type u#4
+// val down4 (p:slprop) : slprop4_base
+// val up4 (p:slprop4_base) : slprop
+// let is_slprop4 (v:slprop) : prop = up4 (down4 v) == v
+// val up4_is_slprop4 (p:slprop4_base) : Lemma (is_slprop4 (up4 p))
 
-(* slprop3: slprops that can be represented in universe 3. *)
-[@@erasable]
-val slprop3_base : Type u#3
-val down3 (p:slprop) : slprop3_base
-val up3 (p:slprop3_base) : slprop
-let is_slprop3 (v:slprop) : prop = up3 (down3 v) == v
-val up3_is_slprop3 (p:slprop3_base) : Lemma (is_slprop3 (up3 p))
+// (* slprop3: slprops that can be represented in universe 3. *)
+// [@@erasable]
+// val slprop3_base : Type u#3
+// val down3 (p:slprop) : slprop3_base
+// val up3 (p:slprop3_base) : slprop
+// let is_slprop3 (v:slprop) : prop = up3 (down3 v) == v
+// val up3_is_slprop3 (p:slprop3_base) : Lemma (is_slprop3 (up3 p))
 
-(* slprop2: slprops that can be represented in universe 2. *)
-[@@erasable]
-val slprop2_base : Type u#2
-val down2 (p:slprop) : slprop2_base
-val up2 (p:slprop2_base) : slprop
-let is_slprop2 (v:slprop) : prop = up2 (down2 v) == v
-val up2_is_slprop2 (p:slprop2_base) : Lemma (is_slprop2 (up2 p))
+// (* slprop2: slprops that can be represented in universe 2. *)
+// [@@erasable]
+// val slprop2_base : Type u#2
+// val down2 (p:slprop) : slprop2_base
+// val up2 (p:slprop2_base) : slprop
+// let is_slprop2 (v:slprop) : prop = up2 (down2 v) == v
+// val up2_is_slprop2 (p:slprop2_base) : Lemma (is_slprop2 (up2 p))
 
-(* slprop1: slprops that can be represented in universe 1. *)
-[@@erasable]
-val slprop1_base : Type u#1
-val down1 (p:slprop) : slprop1_base
-val up1 (p:slprop1_base) : slprop
-let is_slprop1 (v:slprop) : prop = up1 (down1 v) == v
-val up1_is_slprop1 (p:slprop1_base) : Lemma (is_slprop1 (up1 p))
+// (* slprop1: slprops that can be represented in universe 1. *)
+// [@@erasable]
+// val slprop1_base : Type u#1
+// val down1 (p:slprop) : slprop1_base
+// val up1 (p:slprop1_base) : slprop
+// let is_slprop1 (v:slprop) : prop = up1 (down1 v) == v
+// val up1_is_slprop1 (p:slprop1_base) : Lemma (is_slprop1 (up1 p))
 
-let slprop3 = s:slprop { is_slprop3 s }
-let slprop2 = s:slprop { is_slprop2 s }
-let slprop1 = s:slprop { is_slprop1 s }
+// let slprop3 = s:slprop { is_slprop3 s }
+// let slprop2 = s:slprop { is_slprop2 s }
+// let slprop1 = s:slprop { is_slprop1 s }
 
 (* Storable slprops: a storable0 (or storable) can be stored in the heap
 (made into an invariant), and obtain an slprop asserting this fact.
@@ -104,13 +104,13 @@ as an invariant.
 As the heap stack is extended, these names retain their meaning as being
 "N+1" away from the top of the stack. *)
 
-let storable0    = slprop3
-let is_storable0 = is_slprop3
-let storable1    = slprop2
-let is_storable1 = is_slprop2
+// let storable0    = slprop3
+// let is_storable0 = is_slprop3
+// let storable1    = slprop2
+// let is_storable1 = is_slprop2
 
-let storable    = storable0
-let is_storable = is_storable0
+// let storable    = storable0
+// let is_storable = is_storable0
 
 
 //
@@ -124,61 +124,61 @@ let is_storable = is_storable0
 //
 // This is a bit suboptimal
 //
-val slprop_2_is_3 (v:slprop)
-  : Lemma (is_slprop2 v ==> is_slprop3 v)
-          [SMTPat (is_slprop3 v)]
+// val slprop_2_is_3 (v:slprop)
+//   : Lemma (is_slprop2 v ==> is_slprop3 v)
+//           [SMTPat (is_slprop3 v)]
 
-val slprop_1_is_2 (v:slprop)
-  : Lemma (is_slprop1 v ==> is_slprop2 v)
-          [SMTPat (is_slprop2 v)]
+// val slprop_1_is_2 (v:slprop)
+//   : Lemma (is_slprop1 v ==> is_slprop2 v)
+//           [SMTPat (is_slprop2 v)]
 
 val emp : slprop
-val emp_is_slprop2 : squash (is_slprop2 emp)
+// val emp_is_slprop2 : squash (is_slprop2 emp)
 
 val pure (p:prop) : slprop
-val pure_is_slprop2 (p:prop)
-  : Lemma (is_slprop2 (pure p))
-          [SMTPat (is_slprop2 (pure p))]
+// val pure_is_slprop2 (p:prop)
+//   : Lemma (is_slprop2 (pure p))
+        //   [SMTPat (is_slprop2 (pure p))]
 
 val ( ** ) (p q:slprop) : slprop
 
-val slprop3_star (p q : slprop)
-: Lemma
-    (requires is_slprop3 p /\ is_slprop3 q)
-    (ensures is_slprop3 (p ** q))
-    [SMTPat (is_slprop3 (p ** q))]
+// val slprop3_star (p q : slprop)
+// : Lemma
+//     (requires is_slprop3 p /\ is_slprop3 q)
+//     (ensures is_slprop3 (p ** q))
+//     [SMTPat (is_slprop3 (p ** q))]
 
-val slprop2_star (p q : slprop)
-: Lemma
-    (requires is_slprop2 p /\ is_slprop2 q)
-    (ensures is_slprop2 (p ** q))
-    [SMTPat (is_slprop2 (p ** q))]
+// val slprop2_star (p q : slprop)
+// : Lemma
+//     (requires is_slprop2 p /\ is_slprop2 q)
+//     (ensures is_slprop2 (p ** q))
+//     [SMTPat (is_slprop2 (p ** q))]
 
-val slprop1_star (p q : slprop)
-: Lemma
-    (requires is_slprop1 p /\ is_slprop1 q)
-    (ensures is_slprop1 (p ** q))
-    [SMTPat (is_slprop1 (p ** q))]
+// val slprop1_star (p q : slprop)
+// : Lemma
+//     (requires is_slprop1 p /\ is_slprop1 q)
+//     (ensures is_slprop1 (p ** q))
+//     [SMTPat (is_slprop1 (p ** q))]
 
 val ( exists* ) (#a:Type) (p:a -> slprop) : slprop
 
-val slprop3_exists (#a:Type u#a) (p: a -> slprop)
-: Lemma
-    (requires forall x. is_slprop3 (p x))
-    (ensures is_slprop3 (op_exists_Star p))
-    [SMTPat (is_slprop3 (op_exists_Star p))]
+// val slprop3_exists (#a:Type u#a) (p: a -> slprop)
+// : Lemma
+//     (requires forall x. is_slprop3 (p x))
+//     (ensures is_slprop3 (op_exists_Star p))
+//     [SMTPat (is_slprop3 (op_exists_Star p))]
 
-val slprop2_exists (#a:Type u#a) (p: a -> slprop)
-: Lemma
-    (requires forall x. is_slprop2 (p x))
-    (ensures is_slprop2 (op_exists_Star p))
-    [SMTPat (is_slprop2 (op_exists_Star p))]
+// val slprop2_exists (#a:Type u#a) (p: a -> slprop)
+// : Lemma
+//     (requires forall x. is_slprop2 (p x))
+//     (ensures is_slprop2 (op_exists_Star p))
+//     [SMTPat (is_slprop2 (op_exists_Star p))]
 
-val slprop1_exists (#a:Type u#a) (p: a -> slprop)
-: Lemma
-    (requires forall x. is_slprop1 (p x))
-    (ensures is_slprop1 (op_exists_Star p))
-    [SMTPat (is_slprop1 (op_exists_Star p))]
+// val slprop1_exists (#a:Type u#a) (p: a -> slprop)
+// : Lemma
+//     (requires forall x. is_slprop1 (p x))
+//     (ensures is_slprop1 (op_exists_Star p))
+//     [SMTPat (is_slprop1 (op_exists_Star p))]
 
 val slprop_equiv (p q:slprop) : prop
 val elim_slprop_equiv (#p #q:_) (_:slprop_equiv p q) : squash (p == q)
@@ -253,7 +253,7 @@ let slprop_equivs ()
 ////////////////////////////////////////////////////////////////////
 [@@ erasable]
 val iname : Type0
-val storable_iname (i:iname) : GTot bool
+// val storable_iname (i:iname) : GTot bool
 val deq_iname : FStar.GhostSet.decide_eq iname
 instance val non_informative_iname
   : NonInformative.non_informative iname
@@ -271,8 +271,8 @@ let (/!) (is1 is2 : inames) : Type0 =
   GhostSet.disjoint is1 is2
 
 val inv (i:iname) (p:slprop) : slprop
-val storable_inv (i:iname { storable_iname i }) (p:slprop3)
-: Lemma (is_slprop3 (inv i p))
+// val storable_inv (i:iname { storable_iname i }) (p:slprop3)
+// : Lemma (is_slprop3 (inv i p))
 
 let mem_iname (e:inames) (i:iname) : erased bool = elift2 (fun e i -> GhostSet.mem i e) e i
 let mem_inv (e:inames) (i:iname) : GTot bool = mem_iname e i
@@ -585,8 +585,9 @@ val later (p: slprop) : slprop
 val later_intro (p: slprop) : stt_ghost unit emp_inames p fun _ -> later p
 val later_elim (p: slprop) : stt_ghost unit emp_inames (later p ** later_credit 1) fun _ -> p
 
+val timeless (p: slprop) : prop
 (* This is true because ghost functions are called on heaps of nonzero level. *)
-val later_elim_storable (p: storable) : stt_ghost unit emp_inames (later p) fun _ -> p
+val later_elim_timeless (p: slprop { timeless p }) : stt_ghost unit emp_inames (later p) fun _ -> p
 
 //////////////////////////////////////////////////////////////////////////
 // Equivalence
@@ -603,7 +604,7 @@ val equiv_trans a b c : stt_ghost unit emp_inames (equiv a b ** equiv b c) fun _
 val equiv_elim a b : stt_ghost unit emp_inames (a ** equiv a b) fun _ -> b
 
 (* This is true because ghost functions are called on heaps of nonzero level. *)
-val equiv_elim_storable (a b: storable) : stt_ghost unit emp_inames (equiv a b) fun _ -> pure (a == b)
+val equiv_elim_storable (a:slprop { timeless a }) (b: slprop { timeless b }) : stt_ghost unit emp_inames (equiv a b) fun _ -> pure (a == b)
 
 //////////////////////////////////////////////////////////////////////////
 // Higher-order ghost state
@@ -630,8 +631,8 @@ val dup_inv (i:iname) (p:slprop)
 val new_invariant (p:slprop)
 : stt_ghost iname emp_inames p (fun i -> inv i p)
 
-val new_storable_invariant (p:slprop2)
-: stt_ghost (i:iname { storable_iname i }) emp_inames p (fun i -> inv i p)
+// val new_storable_invariant (p:slprop2)
+// : stt_ghost (i:iname { storable_iname i }) emp_inames p (fun i -> inv i p)
 
 val fresh_wrt (i:iname) (c:list iname)
 : prop
@@ -644,7 +645,7 @@ val fresh_wrt_def (i:iname) (c:list iname)
 
 val fresh_invariant
     (ctx:list iname)
-    (p:storable)
+    (p:slprop)
 : stt_ghost (i:iname { i `fresh_wrt` ctx }) emp_inames p (fun i -> inv i p)
 
 val with_invariant
@@ -775,13 +776,13 @@ val pcm_pts_to
     (v:a)
 : slprop
 
-val is_slprop2_pcm_pts_to
-    (#a:Type u#1)
-    (#p:pcm a)
-    (r:pcm_ref p)
-    (v:a)
-: Lemma (is_slprop2 (pcm_pts_to r v))
-        [SMTPat (is_slprop2 (pcm_pts_to r v))]
+// val is_slprop2_pcm_pts_to
+//     (#a:Type u#1)
+//     (#p:pcm a)
+//     (r:pcm_ref p)
+//     (v:a)
+// : Lemma (is_slprop2 (pcm_pts_to r v))
+//         [SMTPat (is_slprop2 (pcm_pts_to r v))]
 
 let pcm_ref_null
     (#a:Type)
@@ -880,13 +881,13 @@ val ghost_pcm_pts_to
     (v:a)
 : slprop
 
-val is_slprop2_ghost_pcm_pts_to
-    (#a:Type u#1)
-    (#p:pcm a)
-    (r:ghost_pcm_ref p)
-    (v:a)
-: Lemma (is_slprop2 (ghost_pcm_pts_to r v))
-        [SMTPat (is_slprop2 (ghost_pcm_pts_to r v))]
+// val is_slprop2_ghost_pcm_pts_to
+//     (#a:Type u#1)
+//     (#p:pcm a)
+//     (r:ghost_pcm_ref p)
+//     (v:a)
+// : Lemma (is_slprop2 (ghost_pcm_pts_to r v))
+//         [SMTPat (is_slprop2 (ghost_pcm_pts_to r v))]
 
 val ghost_alloc
     (#a:Type u#1)
@@ -955,13 +956,13 @@ val big_pcm_pts_to
 : slprop
 
 
-val is_slprop3_big_pcm_pts_to
-    (#a:Type u#2)
-    (#p:pcm a)
-    (r:pcm_ref p)
-    (v:a)
-: Lemma (is_slprop3 (big_pcm_pts_to r v))
-        [SMTPat (is_slprop3 (big_pcm_pts_to r v))]
+// val is_slprop3_big_pcm_pts_to
+//     (#a:Type u#2)
+//     (#p:pcm a)
+//     (r:pcm_ref p)
+//     (v:a)
+// : Lemma (is_slprop3 (big_pcm_pts_to r v))
+//         [SMTPat (is_slprop3 (big_pcm_pts_to r v))]
 
 val big_pts_to_not_null
     (#a:Type)
@@ -1033,13 +1034,13 @@ val big_ghost_pcm_pts_to
     (v:a)
 : slprop
 
-val is_slprop3_big_ghost_pcm_pts_to
-    (#a:Type u#2)
-    (#p:pcm a)
-    (r:ghost_pcm_ref p)
-    (v:a)
-: Lemma (is_slprop3 (big_ghost_pcm_pts_to r v))
-        [SMTPat (is_slprop3 (big_ghost_pcm_pts_to r v))]
+// val is_slprop3_big_ghost_pcm_pts_to
+//     (#a:Type u#2)
+//     (#p:pcm a)
+//     (r:ghost_pcm_ref p)
+//     (v:a)
+// : Lemma (is_slprop3 (big_ghost_pcm_pts_to r v))
+//         [SMTPat (is_slprop3 (big_ghost_pcm_pts_to r v))]
 
 val big_ghost_alloc
     (#a:Type)
